priority.v
@@ -1,6 +1,15 @@
 Add LoadPath "/home/felipec/dev/coq/rt-scheduling-spec".
+Require Import Coq.Arith.Lt.
 Require Import job.
+Require Import helper.
 Require Import schedule.
+
+Definition higher_priority := job -> job -> schedule -> time -> Prop.
+Record valid_priority (hp: higher_priority) : Prop :=
+  { hp_irreflexive: forall (j: job) (sched: schedule) (t: time), ~ hp j j sched t;
+    hp_antisymetric: forall (j1: job) (j2: job) (sched: schedule) (t: time),
+                         hp j1 j2 sched t /\ hp j2 j1 sched t -> j1 = j2
+  }.
 
 Definition fp_order := sporadic_task -> sporadic_task -> Prop.
 
@@ -21,3 +30,26 @@ Definition fixed_priority (hp: higher_priority) (order: fp_order) : Prop :=
                (job_of jhigh tskhigh /\ job_of jlow tsklow /\ fp_higherprio order tskhigh tsklow)
                <-> hp jhigh jlow sched t.
 
+Lemma RM_priority_valid :
+    forall (hp: higher_priority), fixed_priority hp RM -> valid_priority hp.
+Proof.
+    intros.
+    unfold fixed_priority in H.
+    split. intros.
+    specialize (H j j).
+    assert (H0 := excluded_middle (exists tsk, job_of j tsk)).
+    inversion H0. inversion H1 as [tsk].
+    specialize H with tsk tsk sched t.
+    inversion H.
+    assert (H5 := excluded_middle (hp j j sched t)).
+    inversion H5. apply H4 in H6. inversion H6 as [_ [_ H7]].
+    unfold fp_higherprio in H7.
+    inversion H7. unfold RM in H8.
+    assert (H9 := lt_irrefl (task_period tsk)). eauto.
+    assert (H9 := lt_irrefl (task_id tsk)). eauto.
+    apply H6.
+    Admitted. (*TODO finish this proof*)
+
+Definition job_level_fixed_priority (hp: higher_priority) :=
+    forall (sched: schedule) (j1: job) (j2: job) (t: time) (t': time),
+        hp j1 j2 sched t -> hp j1 j2 sched t'.
