liulayland.v
@@ -1,26 +1,58 @@
 Add LoadPath "/home/felipec/dev/coq/rt-scheduling-spec".
 Require Import Coq.Lists.List.
+Require Import Coq.Arith.Lt.
 Require Import job.
 Require Import schedule.
 Require Import identmp.
 Require Import priority.
+Require Import helper.
 
 Section LiuLayland.
+Variable ts: taskset.
 Variable sched: schedule.
 Variable hp: higher_priority.
+Variable arr: arrival_seq.
 Axiom RM_priority : fixed_priority hp RM.
 Axiom uniprocessor : ident_mp 1 sched hp.
+Axiom jobs_from_taskset: schedule_of sched ts.
+Axiom arrival_sequence_from_taskset: ts_arrival_seq ts arr.
 
-Lemma uni_simpler_invariant : forall (jlow : job) (t : time),
-                backlogged jlow sched t <-> exists ! jhigh : job, sched jhigh t = 1.
+Lemma uni_simpler_invariant :
+      forall (jlow : job) (t : time),
+          backlogged jlow sched t
+              <-> exists jhigh : job, hp jhigh jlow sched t /\ sched jhigh t = 1.
 Proof.
   intros.
   assert (H1 := uniprocessor).
   split.
-  intros. unfold backlogged in H. inversion H.
+  intros.
   inversion H1.
   assert (H3 := ident_mp_invariant jlow t).
-  inversion H3.
-
+  inversion H3 as [H4 _]. clear H3 ident_mp_invariant ident_mp_cpus_nonzero. 
+  edestruct ((H4 H) 0). apply le_lt_n_Sm. trivial.
+  inversion H0 as [H5 H6].
+  assert (H7 := element_in_list).
+  specialize (H7 job x (cpumap sched t) 0 H6).
+  specialize (ident_mp_mapping t ).
+  inversion ident_mp_mapping as [_ H8].
+  specialize (H8 x).
+  inversion H8 as [H9 _].
+  specialize (H9 H7).
+  exists x. apply (conj H5 H9).
+  
+  intros. inversion H as [jhigh]. inversion H0.
+  inversion H1.
+  specialize (ident_mp_invariant jlow t).
+  inversion ident_mp_invariant as [_ H4].
+  apply H4.
+  intros. exists jhigh. split. apply H2.
+  specialize (ident_mp_mapping t).
+  inversion ident_mp_mapping as [H6 H7].
+  specialize (H7 jhigh).
+  inversion H7 as [_ H8].
+  apply H8 in H3.
+  clear ident_mp_invariant ident_mp_sched_unit ident_mp_mapping ident_mp_cpus_nonzero H H0 H1 H2 H4 H7 H8.
+  apply In_singleton_list with (x := jhigh); trivial.
+Qed.
 
 End LiuLayland.
